CoqOfRust/core/ops/links/deref.v
@@ -1,0 +1,29 @@
+Require Import CoqOfRust.CoqOfRust.
+Require Import links.M.
+
+Import Run.
+
+(*
+pub trait Deref {
+    type Target: ?Sized;
+    fn deref(&self) -> &Self::Target;
+}
+*)
+Module Deref.
+  Definition Run_deref
+      (Self : Set) `{Link Self}
+      {Target : Set} `{Link Target} :
+      Set :=
+    {deref @
+      IsTraitMethod.t "core::ops::deref::Deref" [] [] (Φ Self) "deref" deref *
+      forall (self : Ref.t Pointer.Kind.Ref Self),
+        {{ deref [] [] [ φ self ] 🔽 Ref.t Pointer.Kind.Ref Target }}
+    }.
+
+  Record Run
+      (Self : Set) `{Link Self}
+      {Target : Set} `{Link Target} :
+      Set := {
+    deref : Run_deref Self (Target := Target);
+  }.
+End Deref.
