CoqOfRust/revm/revm_context_interface/links/host.v
@@ -4,44 +4,21 @@ Require Import CoqOfRust.links.M.
 
 (*
 pub trait Host: TransactionGetter + BlockGetter + CfgGetter {
-    /// Load an account code.
     fn load_account_delegated(&mut self, address: Address) -> Option<AccountLoad>;
-
-    /// Gets the block hash of the given block `number`.
     fn block_hash(&mut self, number: u64) -> Option<B256>;
-
-    /// Gets balance of `address` and if the account is cold.
     fn balance(&mut self, address: Address) -> Option<StateLoad<U256>>;
-
-    /// Gets code of `address` and if the account is cold.
     fn code(&mut self, address: Address) -> Option<Eip7702CodeLoad<Bytes>>;
-
-    /// Gets code hash of `address` and if the account is cold.
     fn code_hash(&mut self, address: Address) -> Option<Eip7702CodeLoad<B256>>;
-
-    /// Gets storage value of `address` at `index` and if the account is cold.
     fn sload(&mut self, address: Address, index: U256) -> Option<StateLoad<U256>>;
-
-    /// Sets storage value of account address at index.
-    ///
-    /// Returns [`StateLoad`] with [`SStoreResult`] that contains original/new/old storage value.
     fn sstore(
         &mut self,
         address: Address,
         index: U256,
         value: U256,
     ) -> Option<StateLoad<SStoreResult>>;
-
-    /// Gets the transient storage value of `address` at `index`.
     fn tload(&mut self, address: Address, index: U256) -> U256;
-
-    /// Sets the transient storage value of `address` at `index`.
     fn tstore(&mut self, address: Address, index: U256, value: U256);
-
-    /// Emits a log owned by `address` with given `LogData`.
     fn log(&mut self, log: Log);
-
-    /// Marks `address` to be deleted, with funds transferred to `target`.
     fn selfdestruct(
         &mut self,
         address: Address,
@@ -50,7 +27,6 @@ pub trait Host: TransactionGetter + BlockGetter + CfgGetter {
 }
 *)
 Module Host.
-  Class Trait (Self : Set) := {
-    (* TODO *)
-  }.
+  (* TODO *)
+  Parameter Run : forall (Self : Set), Set.
 End Host.
