CoqOfRust/revm/revm_interpreter/links/interpreter_InterpreterResult.v
@@ -1,0 +1,23 @@
+Require Import CoqOfRust.CoqOfRust.
+Require Import CoqOfRust.links.M.
+Require Import revm.links.dependencies.
+Require Import revm.revm_interpreter.links.instruction_result.
+Require Import revm_interpreter.links.gas.
+
+Module InterpreterResult.
+  Record t : Set := {
+    result: revm_interpreter.links.instruction_result.InstructionResult.t;
+    output: alloy_primitives.links.bytes_.Bytes.t;
+    gas: revm_interpreter.links.gas.Gas.t;
+  }.
+
+  Global Instance IsLink : Link t := {
+    Φ := Ty.path "revm_interpreter::interpreter::InterpreterResult";
+    φ '(Build_t result output gas) :=
+      Value.StructRecord "revm_interpreter::interpreter::InterpreterResult" [
+        ("result", φ result);
+        ("output", φ output);
+        ("gas", φ gas)
+      ]
+  }.
+End InterpreterResult.
