CoqOfRust/revm/revm_interpreter/instructions/arithmetic.v
@@ -174,7 +174,7 @@ Module instructions.
                         [],
                         [],
                         "popn_top",
-                        [],
+                        [ Value.Integer IntegerKind.Usize 1 ],
                         []
                       |),
                       [
@@ -416,7 +416,7 @@ Module instructions.
                         [],
                         [],
                         "popn_top",
-                        [],
+                        [ Value.Integer IntegerKind.Usize 1 ],
                         []
                       |),
                       [
@@ -658,7 +658,7 @@ Module instructions.
                         [],
                         [],
                         "popn_top",
-                        [],
+                        [ Value.Integer IntegerKind.Usize 1 ],
                         []
                       |),
                       [
@@ -902,7 +902,7 @@ Module instructions.
                         [],
                         [],
                         "popn_top",
-                        [],
+                        [ Value.Integer IntegerKind.Usize 1 ],
                         []
                       |),
                       [
@@ -1190,7 +1190,7 @@ Module instructions.
                         [],
                         [],
                         "popn_top",
-                        [],
+                        [ Value.Integer IntegerKind.Usize 1 ],
                         []
                       |),
                       [
@@ -1424,7 +1424,7 @@ Module instructions.
                         [],
                         [],
                         "popn_top",
-                        [],
+                        [ Value.Integer IntegerKind.Usize 1 ],
                         []
                       |),
                       [
@@ -1712,7 +1712,7 @@ Module instructions.
                         [],
                         [],
                         "popn_top",
-                        [],
+                        [ Value.Integer IntegerKind.Usize 1 ],
                         []
                       |),
                       [
@@ -1942,7 +1942,7 @@ Module instructions.
                         [],
                         [],
                         "popn_top",
-                        [],
+                        [ Value.Integer IntegerKind.Usize 2 ],
                         []
                       |),
                       [
@@ -2189,7 +2189,7 @@ Module instructions.
                         [],
                         [],
                         "popn_top",
-                        [],
+                        [ Value.Integer IntegerKind.Usize 2 ],
                         []
                       |),
                       [
@@ -2361,7 +2361,7 @@ Module instructions.
                         [],
                         [],
                         "popn_top",
-                        [],
+                        [ Value.Integer IntegerKind.Usize 1 ],
                         []
                       |),
                       [
@@ -2789,7 +2789,7 @@ Module instructions.
                         [],
                         [],
                         "popn_top",
-                        [],
+                        [ Value.Integer IntegerKind.Usize 1 ],
                         []
                       |),
                       [
