CoqOfRust/revm/revm_interpreter/instructions/bitwise.v
@@ -174,7 +174,7 @@ Module instructions.
                         [],
                         [],
                         "popn_top",
-                        [],
+                        [ Value.Integer IntegerKind.Usize 1 ],
                         []
                       |),
                       [
@@ -451,7 +451,7 @@ Module instructions.
                         [],
                         [],
                         "popn_top",
-                        [],
+                        [ Value.Integer IntegerKind.Usize 1 ],
                         []
                       |),
                       [
@@ -728,7 +728,7 @@ Module instructions.
                         [],
                         [],
                         "popn_top",
-                        [],
+                        [ Value.Integer IntegerKind.Usize 1 ],
                         []
                       |),
                       [
@@ -1015,7 +1015,7 @@ Module instructions.
                         [],
                         [],
                         "popn_top",
-                        [],
+                        [ Value.Integer IntegerKind.Usize 1 ],
                         []
                       |),
                       [
@@ -1302,7 +1302,7 @@ Module instructions.
                         [],
                         [],
                         "popn_top",
-                        [],
+                        [ Value.Integer IntegerKind.Usize 1 ],
                         []
                       |),
                       [
@@ -1578,7 +1578,7 @@ Module instructions.
                         [],
                         [],
                         "popn_top",
-                        [],
+                        [ Value.Integer IntegerKind.Usize 0 ],
                         []
                       |),
                       [
@@ -1843,7 +1843,7 @@ Module instructions.
                         [],
                         [],
                         "popn_top",
-                        [],
+                        [ Value.Integer IntegerKind.Usize 1 ],
                         []
                       |),
                       [
@@ -2094,7 +2094,7 @@ Module instructions.
                         [],
                         [],
                         "popn_top",
-                        [],
+                        [ Value.Integer IntegerKind.Usize 1 ],
                         []
                       |),
                       [
@@ -2345,7 +2345,7 @@ Module instructions.
                         [],
                         [],
                         "popn_top",
-                        [],
+                        [ Value.Integer IntegerKind.Usize 1 ],
                         []
                       |),
                       [
@@ -2596,7 +2596,7 @@ Module instructions.
                         [],
                         [],
                         "popn_top",
-                        [],
+                        [ Value.Integer IntegerKind.Usize 0 ],
                         []
                       |),
                       [
@@ -2843,7 +2843,7 @@ Module instructions.
                         [],
                         [],
                         "popn_top",
-                        [],
+                        [ Value.Integer IntegerKind.Usize 1 ],
                         []
                       |),
                       [
@@ -3384,7 +3384,7 @@ Module instructions.
                         [],
                         [],
                         "popn_top",
-                        [],
+                        [ Value.Integer IntegerKind.Usize 1 ],
                         []
                       |),
                       [
@@ -3897,7 +3897,7 @@ Module instructions.
                         [],
                         [],
                         "popn_top",
-                        [],
+                        [ Value.Integer IntegerKind.Usize 1 ],
                         []
                       |),
                       [
@@ -4412,7 +4412,7 @@ Module instructions.
                         [],
                         [],
                         "popn_top",
-                        [],
+                        [ Value.Integer IntegerKind.Usize 1 ],
                         []
                       |),
                       [
