CoqOfRust/revm/revm_interpreter/instructions/control.v
@@ -536,7 +536,7 @@ Module instructions.
                         [],
                         [],
                         "popn",
-                        [],
+                        [ Value.Integer IntegerKind.Usize 1 ],
                         []
                       |),
                       [
@@ -937,7 +937,7 @@ Module instructions.
                         [],
                         [],
                         "popn",
-                        [],
+                        [ Value.Integer IntegerKind.Usize 1 ],
                         []
                       |),
                       [
@@ -1412,7 +1412,7 @@ Module instructions.
                         [],
                         [],
                         "popn",
-                        [],
+                        [ Value.Integer IntegerKind.Usize 1 ],
                         []
                       |),
                       [
@@ -1626,7 +1626,7 @@ Module instructions.
                         [],
                         [],
                         "popn",
-                        [],
+                        [ Value.Integer IntegerKind.Usize 2 ],
                         []
                       |),
                       [
@@ -3990,7 +3990,7 @@ Module instructions.
                         [],
                         [],
                         "popn",
-                        [],
+                        [ Value.Integer IntegerKind.Usize 2 ],
                         []
                       |),
                       [
